Qed first lease example

src/program_proof/minlease/proof.v
@@ -6,6 +6,7 @@ From Perennial.base_logic.lib Require Import ghost_var.
 From Goose.github_com.mit_pdos.gokv Require Import minlease.
 From iris.bi.lib Require Import fixpoint.
 From Perennial.base_logic Require Import lib.saved_prop.
+From Perennial.program_proof Require Import std_proof.
 
 Section proof.
 
@@ -28,6 +29,7 @@ Definition underLease (N:namespace) (leaseExpiration:u64) (P:iProp Σ) (Q:iProp 
     (P' ∗ (P' -∗ Q) ∨ is_time_lb leaseExpiration ∗ ghost_var γpostLeastTok 1 ())
   ).
 
+(* Doesn't seem useful
 Lemma underLease_mono P' P Q e N :
   (P -∗ P') -∗
   (P' -∗ Q) -∗
@@ -35,7 +37,7 @@ Lemma underLease_mono P' P Q e N :
   underLease N e P' Q
 .
 Proof.
-Admitted.
+Admitted. *)
 
 Lemma lease_acc_update N e P Q :
   underLease N e P Q -∗
@@ -86,26 +88,26 @@ Definition postLease (N:namespace) (leaseExpiration:u64) (Q:iProp Σ) : iProp Σ
   is_time_lb leaseExpiration ={↑N}=∗ ▷ Q
 .
 
-Lemma lease_alloc N e P :
-  P ={↑N}=∗
-  underLease N e P P ∗
-  postLease N e P
+Lemma lease_alloc e Q N P :
+  P -∗ (P -∗ Q) ={↑N}=∗
+  underLease N e P Q ∗
+  postLease N e Q
 .
 Proof.
-  iIntros "HP".
+  iIntros "HP Hwand".
   iMod (saved_prop_alloc P (DfracOwn 1)) as (γprop) "[Hprop Hprop2]".
   { done. }
   iMod (ghost_var_alloc ()) as (γpostLeaseTok) "HpostLeaseTok".
   iAssert (|={↑N}=>
   inv N (∃ P',
     saved_prop_own γprop (DfracOwn (1/2)) P' ∗
-    (P' ∗ (P' -∗ P) ∨ is_time_lb e ∗ ghost_var γpostLeaseTok 1 ())
-  ))%I with "[HP Hprop2]" as ">#Hinv".
+    (P' ∗ (P' -∗ Q) ∨ is_time_lb e ∗ ghost_var γpostLeaseTok 1 ())
+  ))%I with "[HP Hwand Hprop2]" as ">#Hinv".
   {
     iMod (inv_alloc with "[-]") as "$"; last done.
     iNext.
     iExists _; iFrame "Hprop2".
-    iLeft. iFrame "HP". iIntros "$".
+    iLeft. iFrame.
   }
   iModIntro.
   iSplitL "Hprop".
@@ -138,22 +140,349 @@ Qed.
  *)
 
 Definition own_Server s γ : iProp Σ :=
-  ∃ (v:u64) (leaseExpiration:u64),
+  ∃ (v:u64),
   "Hval" ∷ s ↦[Server :: "val"] #v ∗
-  "HleaseExpiration" ∷ s ↦[Server :: "leaseExpiration"] #leaseExpiration ∗
   "Hauth" ∷ ghost_var γ (1/2) v
 .
+
+
+Definition LEASE_EXP := U64 10.
+
+Definition minleaseN := nroot .@ "minlease".
 
 Definition is_Server s γ : iProp Σ :=
   ∃ mu,
   "#Hmu" ∷ readonly (s ↦[Server :: "mu"] mu) ∗
-  "#HmuInv" ∷ is_lock nroot mu (own_Server s γ)
+  "#HleaseExpiration" ∷ readonly (s ↦[Server :: "leaseExpiration"] #LEASE_EXP) ∗
+  "#HmuInv" ∷ is_lock minleaseN mu (own_Server s γ)
 .
 
-Definition clientPre s γ : iProp Σ :=
-  ∃ mu,
-  "#Hmu" ∷ readonly (s ↦[Server :: "mu"] mu) ∗
-  "#HmuInv" ∷ is_lock nroot mu (own_Server s γ)
+Lemma wp_Put s (v:u64) γ Φ :
+is_Server s γ -∗
+(|={⊤,∅}=> ∃ (oldv:u64), ghost_var γ (1/2) oldv ∗
+(ghost_var γ (1/2) v ={∅,⊤}=∗ Φ #()) )-∗
+  WP Server__Put #s #v {{ Φ }}
 .
+Proof.
+  iIntros "Hsrv Hupd".
+  iNamed "Hsrv".
+  wp_lam.
+  wp_pures.
+  wp_loadField.
+  wp_apply (acquire_spec with "HmuInv").
+  iIntros "[Hlocked Hown]".
+  iNamed "Hown".
+  wp_pures.
+  wp_storeField.
+  wp_loadField.
+
+  iApply fupd_wp.
+  iMod "Hupd" as (?) "[Hval2 Hupd]".
+  iMod (ghost_var_update_2 with "Hauth Hval2") as "[Hauth Hval2]".
+  { apply Qp.half_half. }
+  iMod ("Hupd" with "Hval2") as "HΦ".
+  iModIntro.
+  wp_apply (release_spec with "[-HΦ]").
+  {
+    iFrame "HmuInv Hlocked".
+    iNext.
+    repeat iExists _; iFrame "∗#%".
+  }
+  wp_pures.
+  by iFrame.
+Qed.
+
+Lemma wp_Get s γ Φ :
+is_Server s γ -∗
+(|={⊤,∅}=> ∃ (v:u64), ghost_var γ (1/2) v ∗
+(ghost_var γ (1/2) v ={∅,⊤}=∗ Φ #v) )-∗
+  WP Server__Get #s {{ Φ }}
+.
+Proof.
+  iIntros "Hsrv Hupd".
+  iNamed "Hsrv".
+  wp_lam.
+  wp_pures.
+  wp_loadField.
+  wp_apply (acquire_spec with "HmuInv").
+  iIntros "[Hlocked Hown]".
+  iNamed "Hown".
+  wp_pures.
+  wp_loadField.
+  wp_loadField.
+
+  iApply fupd_wp.
+  iMod "Hupd" as (?) "[Hval2 Hupd]".
+  iDestruct (ghost_var_valid_2 with "Hauth Hval2") as %[_ ->].
+  iMod ("Hupd" with "Hval2") as "HΦ".
+  iModIntro.
+  wp_apply (release_spec with "[-HΦ]").
+  {
+    iFrame "HmuInv Hlocked".
+    iNext.
+    repeat iExists _; iFrame "∗#%".
+  }
+  wp_pures.
+  by iFrame.
+Qed.
+
+Lemma wp_StartServer γ :
+  {{{
+      "Hlease" ∷ underLease minleaseN LEASE_EXP (ghost_var γ (1/2) (U64 0)) (∃ (v:u64), (ghost_var γ (1/2) v)) ∗
+      "Hauth" ∷ ghost_var γ (1/2) (U64 0)
+  }}}
+    StartServer #()
+  {{{
+        s, RET #s; is_Server s γ
+  }}}
+.
+Proof.
+  iIntros (Φ) "Hpre HΦ".
+  iNamed "Hpre".
+  wp_lam.
+  wp_apply (wp_allocStruct).
+  { repeat constructor. }
+  iIntros (?) "Hl".
+  iDestruct (struct_fields_split with "Hl") as "HH".
+  iNamed "HH".
+  wp_pures.
+  wp_apply (wp_new_free_lock).
+  iIntros (mu) "HmuInv".
+  wp_storeField.
+  wp_storeField.
+  wp_storeField.
+  iMod (readonly_alloc_1 with "mu") as "#Hmu".
+  iMod (readonly_alloc_1 with "leaseExpiration") as "#HleaseExpiration".
+
+  iAssert (|={⊤}=> is_Server l γ)%I with "[-HΦ Hlease]" as ">#Hsrv".
+  {
+    repeat iExists _.
+    iFrame "∗#%".
+    iDestruct (alloc_lock with "HmuInv [-]") as "$".
+    iNext.
+    repeat iExists _; iFrame "∗#%".
+  }
+
+  wp_apply (wp_fork with "[-HΦ]").
+  {
+    iNext.
+    wp_pure1_credit "Hlc1".
+    wp_pure1_credit "Hlc2".
+    wp_pures.
+    iAssert  ( ∃ v,
+      "Hlease" ∷ underLease minleaseN LEASE_EXP (ghost_var γ (1 / 2) v%Z)
+               (∃ v' : u64, ghost_var γ (1 / 2) v')
+               )%I with "[Hlease]" as "HH" .
+    { iExists _. iFrame. }
+    wp_forBreak_cond.
+    wp_pures.
+    wp_lam.
+    iClear "Hmu HleaseExpiration".
+    iNamed "Hsrv".
+    wp_loadField.
+    wp_apply (acquire_spec with "HmuInv").
+    iIntros "[Hlocked Hown]".
+    wp_pures.
+    wp_apply (wp_GetTimeRange γtime).
+    iIntros (low high t) "%Hineq1 %Hineq2 Htime".
+    iNamed "HH".
+
+    destruct (decide (int.nat LEASE_EXP < int.nat high)).
+    2:{ (* case: lease is not expired *)
+      iDestruct (lease_acc_update with "Hlease Hlc1 Hlc2") as "HH".
+      iDestruct ("HH" $! t with "[%] Htime") as "HH".
+      { word. }
+      iMod (fupd_mask_subseteq _) as "Hmask"; last iMod "HH".
+      { set_solver. }
+      iNamed "Hown".
+      iDestruct "HH" as "[Hval2 HcloseLease]".
+      iDestruct (ghost_var_valid_2 with "Hauth Hval2") as %[_ ->].
+      iMod (ghost_var_update_2 (word.add v 1) with "Hauth Hval2") as "[Hauth Hval2]".
+      { apply Qp.half_half. }
+
+      iMod ("HcloseLease" $!_ with "Hval2 []") as "[Htime Hlease]".
+      {
+        iIntros. iExists _; iFrame.
+      }
+      iMod "Hmask".
+      iModIntro.
+      iFrame "Htime".
+      wp_pure1_credit "Hlc1".
+      wp_pure1_credit "Hlc2".
+      wp_loadField.
+      wp_pures.
+      wp_bind (If (#(bool_decide _)) _ _).
+      wp_if_destruct.
+      1:{
+        exfalso.
+        word.
+      }
+      wp_loadField.
+      wp_apply (wp_SumAssumeNoOverflow).
+      iIntros "%Hoverflow".
+      wp_storeField.
+      wp_loadField.
+      wp_apply (release_spec with "[-Hlease Hlc1 Hlc2]").
+      {
+        iFrame "HmuInv Hlocked".
+        repeat iExists _; iFrame "∗#%".
+      }
+      wp_pures.
+      iLeft.
+      iModIntro.
+      iSplitR; first done.
+      iFrame.
+      iExists _.
+      iFrame.
+    }
+    (* Otherwise, lease has expired *)
+    iModIntro.
+    iFrame.
+    wp_pures.
+    wp_loadField.
+    wp_pures.
+    wp_bind (If (#(bool_decide _)) _ _).
+    wp_if_destruct.
+    2:{ exfalso. word. }
+    wp_loadField.
+    wp_apply (release_spec with "[-Hlease]").
+    {
+      iFrame "HmuInv Hlocked". iFrame.
+    }
+    wp_pures.
+    iRight.
+    iModIntro.
+    done.
+  }
+  wp_pures.
+  iModIntro.
+  iApply "HΦ".
+  done.
+Qed.
+
+Lemma wp_client s γ :
+  {{{
+      "#Hsrv" ∷ is_Server s γ ∗
+      "HpostLease" ∷ postLease minleaseN LEASE_EXP (∃ (v':u64), ghost_var γ (1/2) v')
+  }}}
+    client #s
+  {{{
+      RET #(); True
+  }}}
+.
+Proof.
+  iIntros (Φ) "Hpre HΦ".
+  iNamed "Hpre".
+  wp_call.
+  wp_forBreak.
+  wp_pures.
+  wp_apply (wp_GetTimeRange γtime).
+  iIntros (low high t Hineq1 Hineq) "Htime".
+
+  iAssert (_) with "Hsrv" as "Hsrv2".
+  iNamed "Hsrv2".
+
+  destruct (decide (int.nat LEASE_EXP < int.nat low)).
+  {
+    iDestruct (mono_nat_lb_own_get with "Htime") as "#Hlb".
+    unfold postLease.
+    iMod (fupd_mask_subseteq _) as "Hmask";
+      last iMod ("HpostLease" with "[Hlb]") as "HpostLease".
+    { set_solver. }
+    { iApply mono_nat_lb_own_le; last iFrame "#". word. }
+    iMod "Hmask" as "_".
+    iModIntro.
+    iFrame "Htime".
+    wp_pures.
+    iDestruct "HpostLease" as (?) "Hghost".
+    wp_loadField.
+    wp_pures.
+    wp_if_destruct.
+    2:{ exfalso. word. }
+    iModIntro.
+    iRight.
+    iSplitR; first done.
+    wp_pures.
+    wp_apply (wp_Get with "Hsrv").
+    iApply fupd_mask_intro.
+    { set_solver. }
+    iIntros "Hmask".
+    iExists _; iFrame.
+    iIntros "Hvar".
+    iMod "Hmask" as "_".
+    iModIntro.
+    wp_pures.
+    wp_apply wp_SumAssumeNoOverflow.
+    iIntros (HnoOverflow).
+    wp_pures.
+    wp_apply (wp_Put with "Hsrv").
+    iApply fupd_mask_intro.
+    { set_solver. }
+    iIntros "Hmask".
+    iExists _; iFrame.
+    iIntros "Hvar".
+    iMod "Hmask" as "_".
+    iModIntro.
+    wp_pures.
+    wp_apply (wp_Get with "Hsrv").
+    iApply fupd_mask_intro.
+    { set_solver. }
+    iIntros "Hmask".
+    iExists _; iFrame.
+    iIntros "Hvar".
+    iMod "Hmask" as "_".
+    iModIntro.
+    wp_pures.
+    wp_apply (wp_Assert).
+    { apply bool_decide_true. done. }
+    wp_pures.
+    iModIntro.
+    by iApply "HΦ".
+  }
+  { (* loop and wait for server's lease to expire *)
+    iFrame "Htime".
+    iModIntro.
+    wp_pures.
+    wp_loadField.
+    wp_pures.
+    wp_if_destruct.
+    { exfalso. word. }
+    wp_loadField.
+    wp_apply wp_Sleep.
+    wp_pures.
+    iLeft.
+    iFrame.
+    done.
+  }
+Qed.
+
+Lemma wp_main :
+  {{{
+       True
+  }}}
+    main #()
+  {{{
+        RET #(); True
+  }}}
+.
+Proof using Type* γtime.
+  iIntros (Φ) "_ HΦ".
+  wp_lam.
+  iMod (ghost_var_alloc (U64 0)) as (γ) "[Hvar Hvar2]".
+  iApply fupd_wp.
+  iMod (fupd_mask_subseteq (↑minleaseN)) as "Hmask".
+  { set_solver. }
+  iMod (lease_alloc LEASE_EXP (∃ v:u64, ghost_var γ (1/2) v) with "Hvar2 []") as "[Hlease HpostLease]".
+  { iIntros. iExists _; iFrame. }
+  iMod "Hmask".
+  iModIntro.
+  wp_apply (wp_StartServer with "[$Hlease $Hvar]").
+  iIntros (s) "#Hsrv".
+  wp_pures.
+  wp_apply (wp_client with "[$Hsrv $HpostLease]").
+  wp_pures.
+  iModIntro.
+  by iApply "HΦ".
+Qed.
 
 End proof.
